added stack.v

Semantics.v
@@ -9,24 +9,8 @@ From Repl Require Import
 
 Inductive result : Type :=
 | success (gs : list goal)
-(* | failure - took out to have multiple types of errors *) 
-(* added two types of failer recoverable vs irrecoverable*)
-| recoverableErr (* "TODO" not sure if we need to add exception as a parameter here
-- did not add it currently because we do not need to throw an exception*)
+| recoverableErr (e : exception) 
 | irrecoverable (e: exception). 
-
-(* "Other TODO"  
--look through stlc chapter about substitution, 
-- adding throw in result for irrecoverable type of plus
-- ignore exn type assume second tactic is always done (tbh 
-I do not remember why)
-*)
-(* also look possibly look at imp *)
-(* | unit (u : unit ) *)
-
-(* Definition thunk := unit -> a. *)
-(* Definition thunk := unit -> result. *)
-
 
 Parameter run_atomic : atomic -> goal -> result.
 
@@ -34,50 +18,36 @@ Inductive execute_atomic : atomic -> goal -> result -> Prop :=
 | e_atomic : forall a g,
   execute_atomic a g (run_atomic a g).
 
-  (* Definition execute_thunk (t : thunk) : result :=
-    t. *)
-
-
 Inductive execute_tactic : tactic -> goal -> result -> Prop :=
 | e_single : forall a g out,
   execute_atomic a g out ->
   execute_tactic (single a) g out
 | e_zero : forall g e ,
-  execute_tactic (zero e) g (recoverableErr) 
-| e_plus_okay1 : forall t1 t2 g outl1,
+  execute_tactic (zero e) g (recoverableErr e ) 
+| e_plus_okay1 : forall t1 x t2 g outl1,
   execute_tactic t1 g (success outl1) ->
-  execute_tactic (plus t1 t2) g (success outl1)
-| e_plus_okay2 : forall t1 t2 g outl2,
-  execute_tactic t1 g (recoverableErr ) ->
-  execute_tactic t2 g outl2 ->
-  execute_tactic (plus t1 t2) g (outl2)
+  execute_tactic (plus t1 x t2) g (success outl1)
+| e_plus_okay2 : forall t1 x t2 g outl2 e,
+  execute_tactic t1 g (recoverableErr e) ->
+  execute_tactic (subst_tactic t2 x e) g outl2 ->
+  execute_tactic (plus t1 x t2) g (outl2)
 | e_throw : forall e g , 
 execute_tactic (throw e) g (irrecoverable e ) 
-(* "TODO" | create a new definition to take in here.
-Would this be  having a irrecoverableErr in the first opening of plus? *)
-| e_plus_notOkay1 : forall t1 t2 g e ,
+| e_plus_notOkay1 : forall t1 t2 g e x ,
 execute_tactic t1 g (irrecoverable e) ->
-execute_tactic (plus t1 t2) g (irrecoverable e). 
-
-
-(* Ensuring backtracking on plus, 
-with recoverable error/failure on first tactics *)
-Goal forall t1 t2 g outl2,
-  execute_tactic t1 g (recoverableErr ) ->
-  execute_tactic t2 g (success outl2) ->
-  execute_tactic (plus t1 t2) g (success outl2).
-Proof.
-intros t1 t2 g out H1 H2.
-apply e_plus_okay2.
-- apply H1. 
-- apply H2.
-Qed.   
+execute_tactic (plus t1 x t2) g (irrecoverable e)
+| tMatch_t1okay : forall t1 t2 g out , 
+  execute_tactic t1 g out -> 
+  execute_tactic (tMatch exn_f1 t1 t2) g out
+| tMatch_t2okay : forall t1 t2 g out,
+  execute_tactic t2 g out -> 
+  execute_tactic (tMatch exn_f2 t1 t2) g out.
 
 (* Test if proof will only output first tactic that works *)
-Goal forall t1 t2 g outl1 outl2,
+Goal forall t1 t2 g x outl1 outl2,
 execute_tactic t1 g (success outl1) ->
 execute_tactic t2 g (success outl2) ->
-execute_tactic (plus t1 t2) g (success outl1).
+execute_tactic (plus t1 x t2) g (success outl1).
 Proof.
 intros. 
 apply e_plus_okay1. apply H.
@@ -85,21 +55,46 @@ Qed.
 
 (* "NEW" ensure that the success t2 will not be
  execute if t1 an irrecoverable error*)
-Goal forall t1 t2 g outl2 e,
+Goal forall t1 t2 g outl2 e x ,
 execute_tactic t1 g(irrecoverable e ) ->
 execute_tactic t2 g (success outl2) ->
-execute_tactic (plus t1 t2) g (irrecoverable e). 
+execute_tactic (plus t1 x t2) g (irrecoverable e). 
 Proof. 
 intros.
 apply e_plus_notOkay1.
 - apply H.
 Qed.    
 
-(* "TODO " trying to figure out how I can create a Goal for throw
-or if it is even conceptually possible*)
-Goal forall e g,
-execute_tactic . 
-Admitted. 
+
+
+Goal forall g t1 t2 t3 out,
+ execute_tactic t1 g (recoverableErr exn_f1)  -> 
+ execute_tactic (subst_tactic t2 "x" exn_f1) g out -> 
+ execute_tactic (plus t1 "x" (tMatch (exn_var "x") t2 t3)) g out.
+Proof. 
+ intros.
+ eapply e_plus_okay2.
+ - eauto.
+ - simpl.
+   apply tMatch_t1okay. eauto.
+Qed.
+
+Goal forall g t1 t2 t3 out,
+ execute_tactic t1 g (recoverableErr exn_f2) ->
+ execute_tactic (subst_tactic t3 "x" exn_f2 ) g out ->
+ execute_tactic (plus t1 "x" (tMatch (exn_var "x") t2 t3)) g out.
+Proof. 
+intros.
+eapply e_plus_okay2.
+- apply H. 
+- simpl. eapply tMatch_t2okay. apply H0.
+Qed. 
+
+
+
+
+
+
 
 
    
