Syntax.v
@@ -11,16 +11,38 @@ Parameter goal : Set.
 
 Inductive exception : Type :=
 (* | exn : string -> exception. *)
-| exn_f1
-| exn_f2
-| exn_var (x: string). 
+| exn_f1 (*fail in the first tactic*)
+| exn_f2 (* fail in the second tactic*)
+| exn_var (x: string). (*specific type of exn? *)
 
 (* Parameter unit : Set.  *)
 
 Inductive tactic : Type := 
 | single (a : atomic)
 | zero (e : exception) (* Ltac2 Documentation: val zero : exn -> 'a*)
-| plus (t1 t2 : tactic) (*Ltac2 documentation: val plus
+| plus (t1 : tactic) ( x: string) (t2 :tactic) (*Ltac2 documentation: val plus
  : (unit -> 'a) -> (exn -> 'a) -> 'a*)
 | throw (e : exception) (*ltac2 documentation: val throw : exn -> 'a*)
-| tMatch (e :exception) (handle1 handle2 : tactic). 
+| tMatch (e :exception) (handle1 handle2 : tactic). (*what is with this implentation?*)
+
+Definition subst_exn (e1 : exception) (x : string) (e2 : exception) : exception :=
+    match e1 with 
+    | exn_f1 => exn_f1
+    | exn_f2 => exn_f2
+    | exn_var x' => if String.eqb x x'
+                        then e2
+                    else e1
+    end. 
+
+Fixpoint subst_tactic (t : tactic) (x : string) (e : exception)  : tactic :=
+    match t with 
+    | single _ => t
+    | zero e' => zero (subst_exn e' x e)
+    | throw e' => throw (subst_exn e' x e)
+    | tMatch e' t1 t2 => tMatch (subst_exn e' x e) (subst_tactic t1 x e) (subst_tactic t2 x e) 
+    | plus t1 x' t2 => if String.eqb x x'
+                            then plus (subst_tactic t1 x e) x' t2
+                        else plus (subst_tactic t1 x e) x' (subst_tactic t2 x e)
+    end. 
+
+    
